some missed changes

pulse/lib/steel/pulse/Pulse.Typing.Metatheory.fst
@@ -1,5 +1,6 @@
 module Pulse.Typing.Metatheory
 open Pulse.Syntax
+open Pulse.Syntax.Naming
 open Pulse.Typing
 
 let st_typing_correctness (#g:env) (#t:st_term) (#c:comp_st) 
@@ -11,4 +12,10 @@ let add_frame_well_typed (#g:env) (#c:comp_st) (ct:comp_typing_u g c)
                          (#f:term) (ft:tot_typing g f Tm_VProp)
   : comp_typing_u g (add_frame c f)
   = admit()
+
+let comp_typing_inversion #g #c ct = admit()
+
+let st_comp_typing_inversion_cofinite (#g:env) (#st:_) (ct:st_comp_typing g st) = admit()
+
+let st_comp_typing_inversion (#g:env) (#st:_) (ct:st_comp_typing g st) = admit()
 
